Compiles

backend/AllocproofC.v
@@ -76,7 +76,7 @@ Hypothesis (WF: SkEnv.wf skenv_link).
 Hypothesis TRANSL: match_prog prog tprog.
 Let ge := (SkEnv.revive (SkEnv.project skenv_link md_src.(Mod.sk)) prog).
 Let tge := (SkEnv.revive (SkEnv.project skenv_link md_tgt.(Mod.sk)) tprog).
-Definition msp: ModSemPair.t := ModSemPair.mk (md_src skenv_link) (md_tgt skenv_link) tt sm_link.
+Definition msp: ModSemPair.t := ModSemPair.mk (md_src skenv_link) (md_tgt skenv_link) (SimSymbId.mk md_src md_tgt) sm_link.
 
 Inductive match_states
           (sm_init: SimMem.t)
@@ -194,7 +194,7 @@ Proof.
     + left. eapply spread_dplus; eauto. eapply modsem_determinate; eauto.
     + instantiate (1:= (SimMemExt.mk _ _)). econs; ss.
 Unshelve.
-  all: ss.
+  all: ss. apply msp.
 Qed.
 
 End SIMMODSEM.
@@ -205,7 +205,7 @@ Section SIMMOD.
 Variable prog: RTL.program.
 Variable tprog: LTL.program.
 Hypothesis TRANSL: match_prog prog tprog.
-Definition mp: ModPair.t := ModPair.mk (RTLC.module2 prog) (LTLC.module tprog) tt.
+Definition mp: ModPair.t := SimSymbId.mk_mp (RTLC.module2 prog) (LTLC.module tprog).
 
 Theorem sim_mod: ModPair.sim mp.
 Proof.
