cfrontend/CstrategyproofC.v
@@ -38,7 +38,7 @@ Hypothesis (INCLTGT: SkEnv.includes skenv_link md_tgt.(Mod.sk)).
 Hypothesis (WF: SkEnv.wf skenv_link).
 Let ge: genv := Build_genv (SkEnv.revive (SkEnv.project skenv_link md_src.(Mod.sk)) prog) prog.(prog_comp_env).
 Let tge: genv := Build_genv (SkEnv.revive (SkEnv.project skenv_link md_tgt.(Mod.sk)) prog) prog.(prog_comp_env).
-Definition msp: ModSemPair.t := ModSemPair.mk (md_src skenv_link) (md_tgt skenv_link) tt sm_link.
+Definition msp: ModSemPair.t := ModSemPair.mk (md_src skenv_link) (md_tgt skenv_link) (SimSymbId.mk md_src md_tgt) sm_link.
 
 Inductive match_states
           (sm_init: SimMem.t)
@@ -107,7 +107,7 @@ End SIMMODSEM.
 Section SIMMOD.
 
 Variables prog: program.
-Definition mp: ModPair.t := ModPair.mk (CsemC.module prog) (module prog).(Mod.Atomic.trans) tt.
+Definition mp: ModPair.t := SimSymbId.mk_mp (CsemC.module prog) (module prog).(Mod.Atomic.trans).
 
 Theorem sim_mod: ModPair.sim mp.
 Proof.
